mppa_k1c/Asmgenproof.v
@@ -40,6 +40,25 @@ Proof.
   exists tp; split. apply Asm.transf_program_match; auto. auto.
 Qed.
 
+(** Return Address Offset *)
+
+Inductive code_tail: Z -> code -> code -> Prop :=
+  | code_tail_0: forall c,
+      code_tail 0 c c
+  | code_tail_S: forall pos i c1 c2,
+      code_tail pos c1 c2 ->
+      code_tail (pos + 1) (i :: c1) c2.
+
+Definition return_address_offset (f: Mach.function) (c: Mach.code) (ofs: ptrofs) : Prop :=
+  forall tf tc,
+  Asmgen.transf_function f = OK tf ->
+  Asmgen.transl_code f c = OK tc ->
+  code_tail (Ptrofs.unsigned ofs) (fn_code tf) tc.
+
+Axiom return_address_exists:
+  forall f sg ros c, is_tail (Mcall sg ros :: c) f.(Mach.fn_code) ->
+  exists ra, return_address_offset f c ra.
+
 Section PRESERVATION.
 
 Variable prog: Mach.program.
@@ -49,7 +68,7 @@ Let ge := Genv.globalenv prog.
 Let tge := Genv.globalenv tprog.
 
 Theorem transf_program_correct:
-  forward_simulation (Mach.semantics (inv_trans_rao return_address_offset) prog) (Asm.semantics tprog).
+  forward_simulation (Mach.semantics return_address_offset prog) (Asm.semantics tprog).
 Proof.
   unfold match_prog in TRANSF. simpl in TRANSF.
   inv TRANSF. inv H. inv H1. inv H. inv H2. inv H.
@@ -61,3 +80,4 @@ Qed.
 End PRESERVATION.
 
 Instance TransfAsm: TransfLink match_prog := pass_match_link (compose_passes block_passes).
+
